utp/utp_parser_utils.thy
@@ -5,7 +5,7 @@
 (* Emails: frank.zeyda@york.ac.uk and simon.foster@york.ac.uk                 *)
 (******************************************************************************)
 
-section {* Parser Utilities *}
+section \<open> Parser Utilities \<close>
 
 theory utp_parser_utils
 imports
@@ -14,8 +14,9 @@ begin
 
 syntax
   "_id_string"     :: "id \<Rightarrow> string" ("IDSTR'(_')")
+  "_id_literal"    :: "id \<Rightarrow> String.literal" ("IDLIT'(_')")
 
-ML {*
+ML \<open>
 signature UTP_PARSER_UTILS =
 sig
   val mk_nib : int -> Ast.ast
@@ -82,15 +83,21 @@ struct
 
   fun mk_id name = Free (name, dummyT);
 end;
-*}
+\<close>
 
-parse_translation {*
+parse_translation \<open>
 let
   fun id_string_tr [Free (full_name, _)] = HOLogic.mk_string full_name
     | id_string_tr [Const (full_name, _)] = HOLogic.mk_string full_name
     | id_string_tr _ = raise Match;
+  fun id_literal_tr [Free (full_name, _)] = HOLogic.mk_literal full_name
+    | id_literal_tr [Const (full_name, _)] = HOLogic.mk_literal full_name
+    | id_literal_tr _ = raise Match;
+
 in
-  [(@{syntax_const "_id_string"}, K id_string_tr)]
+  [(@{syntax_const "_id_string"}, K id_string_tr)
+  ,(@{syntax_const "_id_literal"}, K id_literal_tr)]
 end
-*}
+\<close>
+
 end
